nola/examples/logic/deriv.v
@@ -5,12 +5,12 @@ From iris.proofmode Require Export proofmode.
 
 (** ** [nderivsi]: [derivsi] for [nPropL] *)
 Definition nderivsi Σ `{!nintpGS Σ} : derivsi :=
-  Intpsi (nderivs Σ) (λ d '(Darg i P), ⟦ P ⟧(d)).
+  Intpsi (nderivs Σ) (λ d '(Darg _ P), ⟦ P ⟧(d)).
 
 (** Notation for [nderivsi] *)
 Notation nderivy Σ := (derivy (nderivsi Σ)).
 Notation nderiv := (deriv (ITI:=nderivsi _)).
-Notation ndsound := (dsound (ITI:=nderivsi _)).
+Notation ndsound d := (dsound (ITI:=nderivsi _) d ()).
 Notation nderiv_sound := (deriv_sound (ITI:=nderivsi _)).
 
 (** Utility for [nderiv] *)
@@ -22,14 +22,3 @@ Notation "⟦ P ⟧ˢ" := ⟦ P ⟧ˢ(nderiv) : nola_scope.
 Notation nninv_wsatd := (nninv_wsat nderiv).
 
 Implicit Type P : nPropL (;ᵞ).
-
-(** ** On [nderivy] *)
-Section nderivy.
-  Context `{!nintpGS Σ, !nderivy Σ ih d}.
-
-  (** [d] is monotone over the level *)
-  Lemma derivy_mono_lev {i j P} : i ≤ j → ⸨ P ⸩(d, i) ⊢ ⸨ P ⸩(d, j).
-  Proof.
-    move/Nat.lt_eq_cases=> [?|<-//]. iApply derivy_map_lev; by [|iIntros].
-  Qed.
-End nderivy.
