nola/examples/logic/inv.v
@@ -2,29 +2,25 @@
 
 From nola.examples.logic Require Export deriv.
 
-Implicit Type (i : nat) (P Q : nPropL (;ᵞ)).
+Implicit Type P Q : nPropL (;ᵞ).
 
 Section lemmas.
   Context `{!nintpGS Σ}.
 
   (** Access [nninv] *)
-  Lemma nninv_acc {d i N P E} : ↑N ⊆ E →
-    ndsound d i -∗ nninv d i N P =[nninv_wsat d]{E,E∖↑N}=∗
-      ⟦ P ⟧(d) ∗ (⟦ P ⟧(d) =[nninv_wsat d]{E∖↑N,E}=∗ True).
+  Lemma nninv_acc {N P E} : ↑N ⊆ E →
+    nninvd N P =[nninv_wsatd]{E,E∖↑N}=∗
+      ⟦ P ⟧ ∗ (⟦ P ⟧ =[nninv_wsatd]{E∖↑N,E}=∗ True).
   Proof.
-    rewrite nninv_unseal. iIntros (NE) "to #accP".
+    rewrite nninv_unseal. iIntros (NE) "#accP". iDestruct nderiv_sound as "to".
     iDestruct ("to" with "accP") as "/={accP}accP". by iApply "accP".
   Qed.
-  Lemma nninvd_acc {i N P E} : ↑N ⊆ E →
-    nninvd i N P =[nninv_wsatd]{E,E∖↑N}=∗
-      ⟦ P ⟧ ∗ (⟦ P ⟧ =[nninv_wsatd]{E∖↑N,E}=∗ True).
-  Proof. move=> ?. iApply nninv_acc; [done|iApply nderiv_sound]. Qed.
 
   Context `{!nderivy Σ ih d}.
 
   (** Turn [ninv] into [nninv] *)
-  Lemma ninv_nninv (P : nPropS _) {i N} :
-    ninv N (nInvd_u P) -∗ nninv (Σ:=Σ) d i N (↑ˡ P).
+  Lemma ninv_nninv (P : nPropS _) {N} :
+    ninv N (nInvd_u P) -∗ nninv (Σ:=Σ) d N (↑ˡ P).
   Proof.
     rewrite nninv_unseal. iIntros "#NP !>". iApply (derivy_intro (d:=d))=>/=.
     iIntros (?????). rewrite -nintpS_nintp_nlarge.
@@ -32,29 +28,21 @@ Section lemmas.
   Qed.
 
   (** Allocate [nninv] *)
-  Lemma nninv_alloc_rec (P : nPropS _) {i N} :
-    (nninv d i N (↑ˡ P) -∗ ⟦ P ⟧(d)) =[nninv_wsat d]=∗
-      nninv d i N (↑ˡ P).
+  Lemma nninv_alloc_rec (P : nPropS _) {N} :
+    (nninv d N (↑ˡ P) -∗ ⟦ P ⟧(d)) =[nninv_wsat d]=∗ nninv d N (↑ˡ P).
   Proof.
     iIntros "toP".
     iMod (ninv_alloc_rec (P:=nInvd_u P) with "[toP]") as "NP".
     - iIntros "/=NP". rewrite nintpS_nintp. iApply "toP". by iApply ninv_nninv.
     - iModIntro. by iApply ninv_nninv.
   Qed.
-  Lemma nninv_alloc (P : nPropS _) {i N} :
-    ⟦ P ⟧(d) =[nninv_wsat d]=∗ nninv d i N (↑ˡ P).
+  Lemma nninv_alloc (P : nPropS _) {N} :
+    ⟦ P ⟧(d) =[nninv_wsat d]=∗ nninv d N (↑ˡ P).
   Proof. iIntros "P". iApply (nninv_alloc_rec with "[P]"). by iIntros. Qed.
 
-  (** [nninv] is monotone over the level *)
-  Lemma nninv_mono_lev {i j N P} :
-    i ≤ j → nninv d i N P -∗ nninv d j N P.
-  Proof.
-    rewrite nninv_unseal. iIntros (ij) "#iP !>". by iApply derivy_mono_lev.
-  Qed.
-
   (** Transform [nninv] *)
-  Lemma nninv_convert {i N P Q} :
-    □ ⸨ P ={∅}=∗ Q ∗ (Q ={∅}=∗ P) ⸩(d, i) -∗ nninv d i N P -∗ nninv d i N Q.
+  Lemma nninv_convert {N P Q} :
+    □ ⸨ P ={∅}=∗ Q ∗ (Q ={∅}=∗ P) ⸩(d) -∗ nninv d N P -∗ nninv d N Q.
   Proof.
     rewrite nninv_unseal. iIntros "#PQP #accP !>".
     iApply (derivy_map2 with "[] PQP accP")=>/=.
@@ -65,28 +53,28 @@ Section lemmas.
     iMod (fupd_mask_subseteq ∅) as "toE∖N"; [set_solver|].
     iMod ("QP" with "Q") as "P". iMod "toE∖N" as "_". iApply ("Pto" with "P").
   Qed.
-  Lemma nninv_split {i N P Q} :
-    nninv d i N (P ∗ Q) ⊢ nninv d i N P ∗ nninv d i N Q.
+  Lemma nninv_split {N P Q} :
+    nninv d N (P ∗ Q) ⊢ nninv d N P ∗ nninv d N Q.
   Proof.
     iIntros "#NPQ". iSplit; iApply (nninv_convert with "[] NPQ"); iModIntro;
     iApply (derivy_intro (d:=d)); by iIntros (???) "/=[$$]!>$".
   Qed.
-  Lemma nninv_fupd {i N P} :
-    nninv d i N (|={∅}=> P) ⊣⊢ nninv d i N P.
+  Lemma nninv_fupd {N P} :
+    nninv d N (|={∅}=> P) ⊣⊢ nninv d N P.
   Proof.
     iSplit; iApply nninv_convert; iModIntro; iApply (derivy_intro (d:=d))=>/=;
       iIntros (???); by [iIntros ">$!>$"|iIntros "$!>"; iSplitR; iIntros].
   Qed.
-  Lemma nninv_add {i N P Q} :
-    □ ⸨ P ⸩(d, i) -∗ nninv d i N Q -∗ nninv d i N (P ∗ Q).
+  Lemma nninv_add {N P Q} :
+    □ ⸨ P ⸩(d) -∗ nninv d N Q -∗ nninv d N (P ∗ Q).
   Proof.
     iIntros "#P". iApply nninv_convert. iModIntro.
     iApply (derivy_map with "[] P"). by iIntros (???) "/=$$!>[_$]".
   Qed.
 
   (** Combine [nninv]s *)
-  Lemma nninv_combine {i N N' N'' P Q} : N ## N' → ↑N ∪ ↑N' ⊆@{coPset} ↑N'' →
-    nninv d i N P -∗ nninv d i N' Q -∗ nninv d i N'' (P ∗ Q).
+  Lemma nninv_combine {N N' N'' P Q} : N ## N' → ↑N ∪ ↑N' ⊆@{coPset} ↑N'' →
+    nninv d N P -∗ nninv d N' Q -∗ nninv d N'' (P ∗ Q).
   Proof.
     rewrite nninv_unseal. iIntros (??) "#NP #N'Q !>".
     iApply (derivy_map2 (d:=d) with "[] NP N'Q")=>/=.
