nola/examples/logic/iris.v
@@ -48,12 +48,12 @@ Notation ninv_wsat' intp := (ninv_wsat (nInvd_intp intp)).
 (** ** Derivability structure *)
 
 (** [derivs] for [nPropL] *)
-Definition nderivs Σ : derivs := Intps nat (λ _, nPropL (;ᵞ)) (iProp Σ).
+Definition nderivs Σ : derivs := Intps unit (λ _, nPropL (;ᵞ)) (iProp Σ).
 
 (** Notation for [nderivs] *)
 Notation nderiv_ty Σ := (deriv_ty (nderivs Σ)).
-Notation "⸨ P ⸩ ( d , i )" := (dunwrap d (Darg i P%n))
-  (format "'[' ⸨  P  ⸩ '/  ' ( d ,  i ) ']'") : nola_scope.
+Notation "⸨ P ⸩ ( d )" := (dunwrap d (Darg () P%n))
+  (format "'[' ⸨  P  ⸩ '/  ' ( d ) ']'") : nola_scope.
 
 Section iris.
   Context (* Iris resources *) {Σ : gFunctors}.
@@ -63,27 +63,27 @@ Section iris.
     own γ (to_agree (P : leibnizO _)).
 
   (** [nninv]: [ninv] in the accessor style *)
-  Definition nninv_def (d : nderiv_ty Σ)
-    (i : nat) (N : namespace) (P : nPropL (;ᵞ)) : iProp Σ :=
+  Definition nninv_def (d : nderiv_ty Σ) (N : namespace) (P : nPropL (;ᵞ))
+    : iProp Σ :=
     □ ⸨ ∀ E, ⌜↑N ⊆ E⌝ → |=[n_inv_wsat]{E,E∖↑N}=>
-          P ∗ (P =[n_inv_wsat]{E∖↑N,E}=∗ True) ⸩(d, i).
+          P ∗ (P =[n_inv_wsat]{E∖↑N,E}=∗ True) ⸩(d).
   Definition nninv_aux : seal nninv_def. Proof. by eexists. Qed.
   Definition nninv := nninv_aux.(unseal).
   Lemma nninv_unseal : nninv = nninv_def. Proof. exact nninv_aux.(seal_eq). Qed.
-  #[export] Instance nninv_persistent {d i N P} : Persistent (nninv d i N P).
+  #[export] Instance nninv_persistent {d N P} : Persistent (nninv d N P).
   Proof. rewrite nninv_unseal. exact _. Qed.
 
   (** [na_nninv]: [na_ninv] in the accessor style *)
-  Definition na_nninv_def (d : nderiv_ty Σ) (i : nat)
+  Definition na_nninv_def (d : nderiv_ty Σ)
     (p : na_inv_pool_name) (N : namespace) (P : nPropL (;ᵞ)) : iProp Σ :=
     □ ⸨ ∀ E F, ⌜↑N ⊆ E⌝ → ⌜↑N ⊆ F⌝ → n_na_own p F =[n_inv_wsat]{E}=∗
           P ∗ n_na_own p (F∖↑N) ∗
-          (P -∗ n_na_own p (F∖↑N) =[n_inv_wsat]{E}=∗ n_na_own p F) ⸩(d, i).
+          (P -∗ n_na_own p (F∖↑N) =[n_inv_wsat]{E}=∗ n_na_own p F) ⸩(d).
   Definition na_nninv_aux : seal na_nninv_def. Proof. by eexists. Qed.
   Definition na_nninv := na_nninv_aux.(unseal).
   Lemma na_nninv_unseal : na_nninv = na_nninv_def.
   Proof. exact na_nninv_aux.(seal_eq). Qed.
-  #[export] Instance na_nninv_persistent {d i p N P} :
-    Persistent (na_nninv d i p N P).
+  #[export] Instance na_nninv_persistent {d p N P} :
+    Persistent (na_nninv d p N P).
   Proof. rewrite na_nninv_unseal. exact _. Qed.
 End iris.
