nola/examples/logic/na_inv.v
@@ -2,32 +2,28 @@
 
 From nola.examples.logic Require Export deriv.
 
-Implicit Type (i : nat) (P Q : nPropL (;ᵞ)).
+Implicit Type P Q : nPropL (;ᵞ).
 
 Section lemmas.
   Context `{!nintpGS Σ}.
 
   (** Access [na_nninv] *)
-  Lemma na_nninv_acc {d i p N P E F} : ↑N ⊆ E → ↑N ⊆ F →
-    ndsound d i -∗ na_nninv d i p N P -∗ na_own p F =[nninv_wsat d]{E}=∗
-      ⟦ P ⟧(d) ∗ na_own p (F∖↑N) ∗
-      (⟦ P ⟧(d) -∗ na_own p (F∖↑N) =[nninv_wsat d]{E}=∗ na_own p F).
+  Lemma na_nninv_acc {p N P E F} : ↑N ⊆ E → ↑N ⊆ F →
+    na_nninvd p N P -∗ na_own p F =[nninv_wsatd]{E}=∗
+      ⟦ P ⟧ ∗ na_own p (F∖↑N) ∗
+      (⟦ P ⟧ -∗ na_own p (F∖↑N) =[nninv_wsatd]{E}=∗ na_own p F).
   Proof.
-    rewrite na_nninv_unseal. iIntros (NE NF) "to #accP F".
+    rewrite na_nninv_unseal. iIntros (NE NF) "#accP F".
+    iDestruct nderiv_sound as "to".
     iDestruct ("to" with "accP") as "/={accP}accP".
     iApply ("accP" $! _ _ NE NF with "F").
   Qed.
-  Lemma na_nninvd_acc {i p N P E F} : ↑N ⊆ E → ↑N ⊆ F →
-    na_nninvd i p N P -∗ na_own p F =[nninv_wsatd]{E}=∗
-      ⟦ P ⟧ ∗ na_own p (F∖↑N) ∗
-      (⟦ P ⟧ -∗ na_own p (F∖↑N) =[nninv_wsatd]{E}=∗ na_own p F).
-  Proof. move=> ??. iApply na_nninv_acc; [done..|iApply nderiv_sound]. Qed.
 
   Context `{!nderivy Σ ih d}.
 
   (** Turn [na_ninv] into [na_nninv] *)
-  Lemma na_ninv_nninv (P : nPropS _) {i j p N} : j ∈ (↑N:coPset) →
-    ninv N (nInvd_na p j P) -∗ na_nninv (Σ:=Σ) d i p N (↑ˡ P).
+  Lemma na_ninv_nninv (P : nPropS _) {i p N} : i ∈ (↑N:coPset) →
+    ninv N (nInvd_na p i P) -∗ na_nninv (Σ:=Σ) d p N (↑ˡ P).
   Proof.
     rewrite na_nninv_unseal. iIntros (jN) "#NP !>".
     iApply (derivy_intro (d:=d))=>/=.
@@ -41,33 +37,25 @@ Section lemmas.
   Qed.
 
   (** Allocate [na_nninv] *)
-  Lemma na_nninv_alloc_rec (P : nPropS _) {i p N} :
-    (na_nninv d i p N (↑ˡ P) -∗ ⟦ P ⟧(d)) =[nninv_wsat d]=∗
-      na_nninv d i p N (↑ˡ P).
+  Lemma na_nninv_alloc_rec (P : nPropS _) {p N} :
+    (na_nninv d p N (↑ˡ P) -∗ ⟦ P ⟧(d)) =[nninv_wsat d]=∗
+      na_nninv d p N (↑ˡ P).
   Proof.
-    iIntros "toP". iMod na_lock_alloc as (j) "[% lock]".
-    iMod (ninv_alloc_rec (P:=nInvd_na p j P) with "[toP lock]") as "NP".
+    iIntros "toP". iMod na_lock_alloc as (i) "[% lock]".
+    iMod (ninv_alloc_rec (P:=nInvd_na p i P) with "[toP lock]") as "NP".
     - iIntros "/=NP". iLeft. iFrame "lock". rewrite nintpS_nintp.
       iApply "toP". by iApply na_ninv_nninv.
     - iModIntro. by iApply na_ninv_nninv.
   Qed.
-  Lemma na_nninv_alloc (P : nPropS _) {i p N} :
-    ⟦ P ⟧(d) =[nninv_wsat d]=∗ na_nninv d i p N (↑ˡ P).
+  Lemma na_nninv_alloc (P : nPropS _) {p N} :
+    ⟦ P ⟧(d) =[nninv_wsat d]=∗ na_nninv d p N (↑ˡ P).
   Proof.
     iIntros "P". iApply (na_nninv_alloc_rec with "[P]"). by iIntros.
   Qed.
 
-  (** [na_nninv] is monotone over the level *)
-  Lemma na_nninv_mono_lev {i j p N P} :
-    i ≤ j → na_nninv d i p N P -∗ na_nninv d j p N P.
-  Proof.
-    rewrite na_nninv_unseal. iIntros (ij) "#iP !>". by iApply derivy_mono_lev.
-  Qed.
-
   (** Transform [na_nninv] *)
-  Lemma na_nninv_convert {i p N P Q} :
-    □ ⸨ P ={∅}=∗ Q ∗ (Q ={∅}=∗ P) ⸩(d, i) -∗
-      na_nninv d i p N P -∗ na_nninv d i p N Q.
+  Lemma na_nninv_convert {p N P Q} :
+    □ ⸨ P ={∅}=∗ Q ∗ (Q ={∅}=∗ P) ⸩(d) -∗ na_nninv d p N P -∗ na_nninv d p N Q.
   Proof.
     rewrite na_nninv_unseal. iIntros "#PQP #accP !>".
     iApply (derivy_map2 with "[] PQP accP")=>/=.
@@ -78,29 +66,29 @@ Section lemmas.
     iMod (fupd_mask_subseteq ∅) as "toE∖N"; [set_solver|].
     iMod ("QP" with "Q") as "P". iMod "toE∖N" as "_". iApply ("Pto" with "P").
   Qed.
-  Lemma na_nninv_split {i p N P Q} :
-    na_nninv d i p N (P ∗ Q) ⊢ na_nninv d i p N P ∗ na_nninv d i p N Q.
+  Lemma na_nninv_split {p N P Q} :
+    na_nninv d p N (P ∗ Q) ⊢ na_nninv d p N P ∗ na_nninv d p N Q.
   Proof.
     iIntros "#NPQ". iSplit; iApply (na_nninv_convert with "[] NPQ"); iModIntro;
     iApply (derivy_intro (d:=d)); by iIntros (???) "/=[$$]!>$".
   Qed.
-  Lemma na_nninv_fupd {i p N P} :
-    na_nninv d i p N (|={∅}=> P) ⊣⊢ na_nninv d i p N P.
+  Lemma na_nninv_fupd {p N P} :
+    na_nninv d p N (|={∅}=> P) ⊣⊢ na_nninv d p N P.
   Proof.
     iSplit; iApply na_nninv_convert; iModIntro;
       iApply (derivy_intro (d:=d))=>/=; iIntros (???);
       by [iIntros ">$!>$"|iIntros "$!>"; iSplitR; iIntros].
   Qed.
-  Lemma na_nninv_add {i p N P Q} :
-    □ ⸨ P ⸩(d, i) -∗ na_nninv d i p N Q -∗ na_nninv d i p N (P ∗ Q).
+  Lemma na_nninv_add {p N P Q} :
+    □ ⸨ P ⸩(d) -∗ na_nninv d p N Q -∗ na_nninv d p N (P ∗ Q).
   Proof.
     iIntros "#P". iApply na_nninv_convert. iModIntro.
     iApply (derivy_map with "[] P"). by iIntros (???) "/=$$!>[_$]".
   Qed.
 
   (** Combine [na_nninv]s *)
-  Lemma nninv_combine {i p N N' N'' P Q} : N ## N' → ↑N ∪ ↑N' ⊆@{coPset} ↑N'' →
-    na_nninv d i p N P -∗ na_nninv d i p N' Q -∗ na_nninv d i p N'' (P ∗ Q).
+  Lemma nninv_combine {p N N' N'' P Q} : N ## N' → ↑N ∪ ↑N' ⊆@{coPset} ↑N'' →
+    na_nninv d p N P -∗ na_nninv d p N' Q -∗ na_nninv d p N'' (P ∗ Q).
   Proof.
     rewrite na_nninv_unseal. iIntros (??) "#NP #N'Q !>".
     iApply (derivy_map2 (d:=d) with "[] NP N'Q")=>/=.
