nola/examples/logic/verify/vlist.v
@@ -7,15 +7,15 @@ From nola.examples.heap_lang Require Export notation.
 Fixpoint vlist {κ Γ} (N N' : namespace) (φ : Z → Prop) (ns : list Z) (l : loc)
   : nProp κ Γ :=
   match ns with [] => True | n :: ns =>
-    n_inv 0 N (⌜φ n⌝ ∗ l ↦ # n) ∗
-      n_inv 0 N' (∃ l' : loc, (l +ₗ 1) ↦ # l' ∗ vlist N N' φ ns l') end.
+    n_inv N (⌜φ n⌝ ∗ l ↦ # n) ∗
+      n_inv N' (∃ l' : loc, (l +ₗ 1) ↦ # l' ∗ vlist N N' φ ns l') end.
 
 (** Interpretaion of [vlist] *)
 Definition vlisti `{!nintpGS Σ} d N N' φ (ns : list Z) l
   : iProp Σ :=
   match ns with [] => True | n :: ns =>
-    nninv d 0 N (⌜φ n⌝ ∗ l ↦ # n) ∗
-      nninv d 0 N' (∃ l' : loc, (l +ₗ 1) ↦ # l' ∗ vlist N N' φ ns l') end.
+    nninv d N (⌜φ n⌝ ∗ l ↦ # n) ∗
+      nninv d N' (∃ l' : loc, (l +ₗ 1) ↦ # l' ∗ vlist N N' φ ns l') end.
 Notation vlistis := (vlisti nderiv).
 
 Section verify.
@@ -34,9 +34,9 @@ Section verify.
   Proof.
     move=> ?. move: l. elim ns; [iPureIntro=>/= ??; by apply Forall_nil|].
     iIntros (?? IH ??) "[#ihd #itl]".
-    iMod (nninvd_acc with "ihd") as "/=[[% ↦] cl]"; [done|].
+    iMod (nninv_acc with "ihd") as "/=[[% ↦] cl]"; [done|].
     iMod ("cl" with "[$↦//]") as "_".
-    iMod (nninvd_acc with "itl") as "/=[(%& ↦ & vl) cl]"; [done|].
+    iMod (nninv_acc with "itl") as "/=[(%& ↦ & vl) cl]"; [done|].
     rewrite vlist_vlisti. iDestruct "vl" as "#?". iMod ("cl" with "[↦]") as "_".
     { iExists _. rewrite vlist_vlisti. by iFrame. }
     iMod (IH with "[//]") as %?; [done|]. iPureIntro. by constructor.
